theories/ghost_state.v
@@ -18,6 +18,8 @@ Class heapG Σ := HeapG {
   heap_instrs_inG :> inG Σ instrtblUR;
   heap_instrs_name : gname;
   heap_regs_inG :> ghost_mapG Σ string valu;
+  heap_mem_inG :> ghost_mapG Σ addr byte;
+  heap_mem_name : gname;
   heap_full_trace : list seq_label;
   heap_spec_trace : list seq_label;
   heap_spec_trace_inG :> ghost_varG Σ (list seq_label);
@@ -61,6 +63,27 @@ Section definitions.
   Definition regs_ctx `{!threadG} (regs : reg_map) : iProp Σ :=
     ghost_map_auth thread_regs_name 1 regs.
 
+  Definition mem_mapsto_def (γ : gname) (a : addr) (q : frac) (v : byte) : iProp Σ :=
+    a ↪[ γ ]{# q} v.
+  Definition mem_mapsto_aux : seal (@mem_mapsto_def). by eexists. Qed.
+  Definition mem_mapsto := unseal mem_mapsto_aux.
+  Definition mem_mapsto_eq : @mem_mapsto = @mem_mapsto_def :=
+    seal_eq mem_mapsto_aux.
+
+  Definition mem_ctx (mem : mem_map) : iProp Σ :=
+    ghost_map_auth heap_mem_name 1 mem.
+
+  Fixpoint mem_mapsto_word (a : bv) (len : nat) (w : bv) : iProp Σ :=
+    match len with
+    | 0%nat => ⌜w.(bv_len) = 0 ∧ w.(bv_val) = 0⌝
+    | S n =>
+      let next := bv_add a [BV{64} 1] in
+      let byte := (bv_extract 7 0 w) in
+      let rest := bv_extract (w.(bv_len) - 1) 8 w in
+      mem_mapsto heap_mem_name a.(bv_val) 1 byte ∗
+      mem_mapsto_word next n rest
+    end.
+
   Definition spec_trace_def (κs: list seq_label) : iProp Σ :=
     ghost_var heap_spec_trace_name (1/2) κs.
   Definition spec_trace_aux : seal (@spec_trace_def). by eexists. Qed.
@@ -75,7 +98,8 @@ Section definitions.
 
   Definition state_ctx (σ : seq_global_state) (κs : list seq_label) : iProp Σ :=
     spec_ctx κs ∗
-    instr_ctx σ.(seq_instrs).
+    instr_ctx σ.(seq_instrs) ∗
+    mem_ctx σ.(seq_mem).
 
   Definition thread_ctx `{!threadG} (regs : reg_map) : iProp Σ :=
     regs_ctx regs.
@@ -85,6 +109,11 @@ End definitions.
 Notation "r ↦ᵣ{ q } v" := (reg_mapsto thread_regs_name r q v)
   (at level 20, q at level 50, format "r  ↦ᵣ{ q }  v") : bi_scope.
 Notation "r ↦ᵣ v" := (reg_mapsto thread_regs_name r 1 v) (at level 20) : bi_scope.
+
+
+Notation "a ↦ₘ{ q } v" := (mem_mapsto heap_mem_name a q v)
+  (at level 20, q at level 50, format "a  ↦ₘ{ q }  v") : bi_scope.
+Notation "a ↦ₘ v" := (mem_mapsto heap_mem_name a 1 v) (at level 20) : bi_scope.
 
 Section instr.
   Context `{!heapG Σ}.
@@ -147,6 +176,92 @@ Section reg.
     by iMod (ghost_map_update with "Hregs Hreg") as "[? $]".
   Qed.
 End reg.
+
+Section mem.
+  Context `{!heapG Σ}.
+
+  Global Instance mem_mapsto_tl γ a q v : Timeless (mem_mapsto γ a q v).
+  Proof. rewrite mem_mapsto_eq. by apply _. Qed.
+
+  Lemma mem_mapsto_lookup mem a q v :
+    mem_ctx mem -∗ a ↦ₘ{q} v -∗ ⌜mem !! a = Some v⌝.
+  Proof.
+    rewrite mem_mapsto_eq.
+    iIntros "Hmem Ha".
+    by iDestruct (ghost_map_lookup with "Hmem Ha") as %?.    
+  Qed.
+
+  Lemma mem_mapsto_update mem a v v' :
+    mem_ctx mem -∗ a ↦ₘ v ==∗ mem_ctx (<[a := v']> mem) ∗ a ↦ₘ v'.
+  Proof.
+    iIntros "Hmem Ha".
+    iDestruct (mem_mapsto_lookup with "Hmem Ha") as %?.
+    rewrite mem_mapsto_eq.
+    by iMod (ghost_map_update with "Hmem Ha") as "[? $]".
+  Qed.
+
+  Lemma mem_mapsto_word_lookup mem a len w :
+    mem_ctx mem -∗ mem_mapsto_word a len w -∗ ⌜read_mem mem a len = w⌝.
+  Proof.
+    iIntros "Hmem Ha".
+    iInduction len as [ | n ] "IH" forall (w a).
+    + unfold read_mem.
+      unfold mem_mapsto_word.
+      iDestruct "Ha" as %[Ha1 Ha2].
+      iPureIntro.
+      destruct w.
+      cbn in Ha1.
+      cbn in Ha2.
+      rewrite Ha1 Ha2.
+      done.
+    + cbn.
+      iDestruct "Ha" as "[Hbyte Hrest]".
+      iDestruct (mem_mapsto_lookup with "Hmem Hbyte") as %?.
+      rewrite H.
+      set (next:=(bv_add a [BV{64} 1])).
+      iDestruct ("IH" with "Hmem Hrest") as "H".
+      iDestruct "H" as %G.
+      rewrite G.
+      iPureIntro.
+      apply (bv_concat_split 7 w).
+  Qed.
+
+  Definition rest (w : bv) := bv_extract (bv_len w - 1) 8 w.
+
+  Lemma len_rest (w : bv) : bv_len (rest w) = bv_len w - 8.
+  Proof.
+    cbn.
+    lia.
+  Qed.
+
+  Lemma mem_mapsto_word_update mem a len w w' :
+    ⌜w.(bv_len) = w'.(bv_len)⌝ -∗ mem_ctx mem -∗ mem_mapsto_word a len w ==∗
+    mem_ctx (write_mem mem a w' len) ∗ mem_mapsto_word a len w'.
+  Proof.
+    iIntros "Hlen Hmem Ha".
+    iInduction len as [ | n ] "IH" forall (w w' a mem).
+    + cbn.
+      iModIntro. iFrame.
+      iDestruct "Hlen" as %Hlen.
+      iDestruct "Ha" as %[Hwlen Hwval].
+      iPureIntro; split. { rewrite <- Hlen. assumption. }
+      apply bv_zero_len. rewrite <- Hlen. assumption.
+    + cbn.
+      iDestruct "Ha" as "[Hbyte Hrest]".
+      fold (rest w) (rest w').
+      iDestruct "Hlen" as %Hlen.
+      iAssert ⌜bv_len (rest w) = bv_len (rest w')⌝%I as "Hlen'".
+      {
+        repeat rewrite len_rest.
+        by rewrite Hlen.
+      }
+      iMod (mem_mapsto_update with "Hmem Hbyte") as "[Hmem Hbyte]".
+      iMod ("IH" with "Hlen' Hmem Hrest") as "[Hmem Hrest]".
+      iModIntro.
+      iFrame.
+  Qed.
+      
+End mem.
 
 Section spec.
   Context `{!heapG Σ}.
